more

thys/MRBNF_FP.thy
@@ -350,9 +350,10 @@ lemma extend_fresh:
 ML \<open>
 local
   open BNF_Util
+  open BNF_FP_Util
 in
 
-fun refreshability_tac B Tsupp G_thm small_thms instss simp_thms intro_thms elim_thms ctxt =
+fun refreshability_tac verbose B Tsupp G_thm small_thms instss simp_thms intro_thms elim_thms extend_thms eqvt_thm ctxt =
   let
     val fresh = infer_instantiate' ctxt
       [SOME (Thm.cterm_of ctxt B),
@@ -362,20 +363,24 @@ fun refreshability_tac B Tsupp G_thm small_thms instss simp_thms intro_thms elim
     fun case_tac NONE _ prems ctxt = SOLVE (auto_tac (ctxt addsimps map (simplify ctxt) prems addSIs map (simplify ctxt) prems))
       | case_tac (SOME insts) params prems ctxt =
         let
-          val prems = map (simplify ctxt) prems;
+          val eqvt_thm = eqvt_thm OF take 2 prems;
+          val extra_thms = prems RL (eqvt_thm :: extend_thms);
+val _ = prems |> map (Thm.pretty_thm ctxt #> verbose ? @{print tracing});
+val _ = extra_thms |> map (Thm.pretty_thm ctxt #> verbose ? @{print tracing});
           val f = hd params |> snd |> Thm.term_of;
           val ex_f = infer_instantiate' ctxt [NONE, SOME (Thm.cterm_of ctxt f)] exI;
           val args = tl params |> map (snd #> Thm.term_of);
           val xs = @{map 2} (fn i => fn a => Thm.cterm_of ctxt (i $ f $ a)) insts args;
           val id_onI = nth prems 4 RS @{thm id_on_antimono};
         in
-          HEADGOAL (EVERY' (map (fn x => rtac ctxt (infer_instantiate' ctxt [NONE, SOME x] exI)) xs)) THEN
-print_tac ctxt "pre_auto" THEN
-          SOLVE (HEADGOAL (SELECT_GOAL (mk_auto_tac (ctxt
-            addsimps (simp_thms @ prems)
-            addSIs (ex_f :: id_onI :: intro_thms)
-            addSEs elim_thms) 0 4) THEN_ALL_NEW
-            SELECT_GOAL (print_tac ctxt "auto failed")))
+          HEADGOAL (EVERY' (map (fn x => rtac ctxt (infer_instantiate' ctxt [NONE, SOME x] exI)) xs) THEN'
+            Method.insert_tac ctxt (prems @ extra_thms) THEN'
+            hyp_subst_tac_thin true ctxt THEN'
+            K (if verbose then print_tac ctxt "pre_auto" else all_tac) THEN'
+            SELECT_GOAL (mk_auto_tac (ctxt
+              addsimps (simp_thms @ prems)
+              addSIs (ex_f :: id_onI :: intro_thms)
+              addSEs elim_thms) 0 4) THEN_ALL_NEW (SELECT_GOAL (print_tac ctxt "auto failed")))
         end;
   in
     HEADGOAL (rtac ctxt (fresh RS exE) THEN'
@@ -385,7 +390,7 @@ print_tac ctxt "pre_auto" THEN
       EVERY' [rtac ctxt exI, rtac ctxt conjI, assume_tac ctxt] THEN'
       rtac ctxt (G_thm RSN (2, cut_rl)) THEN'
       REPEAT_ALL_NEW (eresolve_tac ctxt @{thms exE conjE disj_forward}) THEN'
-      EVERY' (map (fn insts => Subgoal.FOCUS (fn focus =>
+      EVERY' (map (fn insts => Subgoal.SUBPROOF (fn focus =>
         case_tac insts (#params focus) (#prems focus) (#context focus)) ctxt) instss))
   end;
 
