thys/Untyped_Lambda_Calculus/LC_Beta_depth.thy
@@ -26,7 +26,7 @@ binder_inductive stepD
         | ((rule exI[of _ "\<sigma> _"] exI)+, (rule conjI)?, rule refl)
         | ((rule exI[of _ "\<sigma> _"])+; auto))+
   subgoal premises prems for R B d t1 t2
-    apply (tactic \<open>refreshability_tac @{term B} @{term "Tsupp d t1 t2"}
+    by (tactic \<open>refreshability_tac false @{term B} @{term "Tsupp d t1 t2"}
       @{thm prems(3)} @{thms emp_bound singl_bound term.Un_bound term.card_of_FFVars_bounds infinite}
       [SOME [@{term "(\<lambda>f x. f x) :: (var \<Rightarrow> var) \<Rightarrow> var \<Rightarrow> var"},
              @{term "rrename :: (var \<Rightarrow> var) \<Rightarrow> trm \<Rightarrow> trm"},
@@ -38,10 +38,11 @@ binder_inductive stepD
              @{term "rrename :: (var \<Rightarrow> var) \<Rightarrow> trm \<Rightarrow> trm"},
              @{term "(\<lambda>f x. f x) :: (var \<Rightarrow> var) \<Rightarrow> var \<Rightarrow> var"}]]
       @{thms Lam_inject}
-      @{thms prems(2)[simplified] Lam_eq_tvsubst term.rrename_cong_ids[symmetric]}
+      @{thms Lam_eq_tvsubst term.rrename_cong_ids[symmetric]}
       @{thms }
+      @{thms }
+      @{thm prems(2)}
       @{context}\<close>)
-    done
   done
 
 thm stepD.strong_induct
